

Задание:

1. $(\exists x)(\exists y)\phi \equiv (\exists y)(\exists x)\phi$
2. $(\forall x)\phi \equiv (\forall y)(\phi)_y^x$
3. $(\exists x)\phi \rightarrow (\forall x)\psi \vdash (\forall x)(\phi \rightarrow \psi)$

Решение:

$$\begin{array}{c}
 \frac{\phi \vdash \phi}{\phi \vdash (\exists x)\phi} \text{ } \exists \text{ введ. справа)} \\
 \frac{\phi \vdash (\exists x)\phi}{\phi \vdash (\exists y)(\exists x)\phi} \text{ } (\exists \text{ введ. справа)} \\
 \frac{\phi \vdash (\exists y)(\exists x)\phi}{(\exists y)\phi \vdash (\exists y)(\exists x)\phi} \text{ } (\exists \text{ введ. слева)} \\
 \frac{(\exists y)\phi \vdash (\exists y)(\exists x)\phi}{(\exists x)(\exists y)\phi \vdash (\exists y)(\exists x)\phi} \text{ } (\exists \text{ введ. слева)}
 \end{array}$$

$$\text{(b)} \quad \frac{\text{Аналогично.}}{(\exists y)(\exists x)\phi \vdash (\exists x)(\exists y)\phi}$$

$$\begin{array}{c}
 \frac{(\phi)_{yx}^{xy} \vdash \phi}{(\forall y)(\phi)_y^x \vdash \phi} \text{ } (\forall \text{ введ. слева)} \\
 \frac{(\forall y)(\phi)_y^x \vdash \phi}{(\forall y)(\phi)_y^x \vdash (\forall x)\phi} \text{ } (\forall \text{ введ. справа)}
 \end{array}$$

$$\begin{array}{c}
 \frac{(\phi)_y^x \vdash (\phi)_y^x}{(\forall y)\phi \vdash (\phi)_y^x} \text{ } (\forall \text{ введ. слева)} \\
 \frac{(\forall y)\phi \vdash (\phi)_y^x}{(\forall x)\phi \vdash (\forall y)(\phi)_y^x} \text{ } (\forall \text{ введ. справа)}
 \end{array}$$

3.

$$\begin{array}{c}
\frac{\phi \vdash \phi}{\phi \vdash (\exists x)\phi} \quad \frac{(\exists x)\phi \rightarrow (\forall x)\psi \vdash (\exists x)\phi \rightarrow (\forall x)\psi}{(\exists x)\phi \rightarrow (\forall x)\psi, \phi \vdash (\exists x)\phi \rightarrow (\forall x)\psi} \quad \frac{\frac{\phi \vdash \phi}{\neg\phi, \phi, \neg\psi \vdash \phi} \quad \frac{\neg\phi \vdash \neg\phi}{\phi, \neg\phi, \neg\psi \vdash \neg\phi}}{\phi, \neg\phi \vdash \psi} \quad \frac{\psi \vdash \psi}{(\forall x)\psi \vdash \psi} \\
\frac{(\exists x)\phi \rightarrow (\forall x)\psi, \phi \vdash (\exists x)\phi \quad (\exists x)\phi \rightarrow (\forall x)\psi, \phi \vdash (\exists x)\phi \rightarrow (\forall x)\psi}{(\exists x)\phi \rightarrow (\forall x)\psi, \phi \vdash (\forall x)\psi} \quad \frac{\phi, \neg\phi \vdash \psi}{\phi, (\forall x)\neg\phi \vdash \psi} \quad \frac{\psi \vdash \psi}{(\forall x)\psi \vdash \psi} \\
(\rightarrow \text{удал.}) \frac{}{(\exists x)\phi \rightarrow (\forall x)\psi, \phi \vdash (\forall x)\neg\phi \vee (\forall x)\psi} \quad (\forall \text{ введ. слева}) \frac{}{(\exists x)\phi \rightarrow (\forall x)\psi, \phi, (\forall x)\neg\phi \vdash \psi} \quad (\forall \text{ введ. справа}) \frac{}{(\exists x)\phi \rightarrow (\forall x)\psi, \phi, (\forall x)\psi \vdash \psi} \\
(\forall \text{ введ.}) \frac{}{(\exists x)\phi \rightarrow (\forall x)\psi, \phi \vdash (\forall x)\neg\phi \vee (\forall x)\psi} \quad (\text{уточн.}) \frac{}{(\exists x)\phi \rightarrow (\forall x)\psi, \phi, (\forall x)\neg\phi \vdash \psi} \quad (\text{уточн.}) \frac{}{(\exists x)\phi \rightarrow (\forall x)\psi, \phi, (\forall x)\psi \vdash \psi} \\
\frac{(\exists x)\phi \rightarrow (\forall x)\psi, \phi \vdash \psi}{(\exists x)\phi \rightarrow (\forall x)\psi \vdash \phi \rightarrow \psi} \quad (\rightarrow \text{введ.}) \quad \frac{}{(\exists x)\phi \rightarrow (\forall x)\psi \vdash (\forall x)(\phi \rightarrow \psi)} \quad (\forall \text{ введ. справа})
\end{array}$$